main and global declarations

proiect.v
@@ -103,6 +103,7 @@ Check &&"a".
 (*Arrays*)
 
 Inductive Array :=
+| error_array : Array
 | array_nat : string -> list nat -> Array
 | array_bool : string -> list bool -> Array
 | array_string : string -> list string -> Array.
@@ -185,6 +186,7 @@ Inductive Stmt :=
 | pointer_decl: string -> pointer -> Stmt
 | reference_decl : string -> string -> Stmt
 | list_decl : string -> ListOp -> Stmt
+| struct_decl : string -> string -> Stmt
 | nat_assign : string -> AExp -> Stmt
 | bool_assign : string -> BExp -> Stmt
 | string_assign : string -> StringExp -> Stmt
@@ -196,15 +198,15 @@ Inductive Stmt :=
 | while : BExp -> Stmt -> Stmt
 | For : Stmt -> BExp -> Stmt -> Stmt -> Stmt
 | switch : AExp -> list cases -> Stmt
-| functionDeclare: string -> list parameters -> Stmt -> Stmt
-| functionCall: string -> list string -> Stmt
+| functionCall: string -> list parameters -> Stmt
 with cases  :=
 | case : AExp -> Stmt -> cases
 | defaultcase: Stmt -> cases
 with parameters :=
-| nat_param: string -> ErrorNat -> parameters
-| bool_param: string -> ErrorBool -> parameters
-| string_param: string -> ErrorString ->parameters.
+| nat_param : string -> ErrorNat -> parameters
+| bool_param : string -> ErrorBool -> parameters
+| string_param : string -> ErrorString -> parameters
+| variable : string -> parameters.
 
 
 Notation "'Nat'' X ::= A" := (nat_decl X A)(at level 90).
@@ -240,7 +242,7 @@ Check For("a":n=0 ; "a"<'10 ; "a" :n= "a" +' 1)
  }.
 Check "a" :p= nullptr.
 Check array_nat "a" [1;2] [[[1]]].
-Check "func" {{["a"]}}.
+Check "func" {{[variable "a"]}}.
 Check switch (1+'2) [ defaultcase ("a" :n= 5)].
 Check switch (avar "a")
     [case (5) ("a" :n= 4);
@@ -250,6 +252,9 @@ Check switch (avar "a")
 Inductive Value:=
 | undeclared : Value
 | default : Value
+| default_nat : Value
+| default_bool : Value
+| default_string : Value
 | err_assign : Value
 | nat_value : ErrorNat -> Value
 | bool_value : ErrorBool -> Value
@@ -258,29 +263,34 @@ Inductive Value:=
 
 Check code ("a" :n= 0).
 
-(* Struct *)
-Inductive Members :=
-| member: string -> Value -> Members.
 
-Inductive Struct :=
-| nullStr : Struct
-| struct : string -> list Members -> Struct.
+(* Program *)
 
-Definition structEnv := string -> Struct.
+Inductive program :=
+| Seq_prg: program -> program -> program
+| decl_globalNat : string -> AExp -> program
+| decl_globalBool : string -> BExp -> program
+| decl_globalString : string -> StringExp -> program
+| function: string -> list types -> Value -> program
+| struct : string -> list members -> program
+| main: Stmt ->program
+with types :=
+| natural: string -> types
+| bool: string -> types
+| string: string -> types
+with members :=
+| member: string -> Value -> members.
 
-Compute struct "s1" [member "a" default].
-Compute struct "s2" [member "b" (bool_value true); 
-                member "x" (default)].
+Notation " A ;;; B " := (Seq_prg A B)(at level 20).
+Notation "'Nat_gl' A ::n= B" := (decl_globalNat A B)(at level 30).
+Notation "'Bool_gl' A ::b= B" := (decl_globalBool A B)(at level 30).
+Notation "'String_gl' A ::s= B" := (decl_globalString A B)(at level 30).
+(* Notation "'func' A '(' B ')' '{(' C ')}' 'end_func'" := (function A B C)(at level 100). *)
 
-Definition structEnv1 : structEnv := fun x => nullStr.
-
-(* update_structEnv*)
-
-Definition declareStruct (s:string) (l:(list Members)) : Struct :=
-match structEnv1 s with
-| struct a b=> struct s l
-| nullStr => nullStr
-end.
+Check main ("a" :n= 10) ;;; function "f1" [natural "a"] (code ("a" :n=10)).
+Check Nat_gl "a" ::n= 10.
+Check Bool_gl "b" ::b= btrue.
+Check String_gl "s" ::s= "start"%string.
 
 
 Check "n" :n= 10 ;;
@@ -288,7 +298,7 @@ Check "n" :n= 10 ;;
       "i" :n= 0 ;;
       "msg" :s= "Hello" ;;
 
-      "func" {{["a"]}};;
+      "func" {{[variable "a"]}};;
       switch (avar "a")
      [case (5) ("a" :n= 4);
      defaultcase ("a" :n= 0)];;
@@ -297,468 +307,39 @@ Check "n" :n= 10 ;;
             "i" :n= "i" +' 1
       ).
 
+Definition prg := 
+  (Nat_gl "sum" ::n= 0) ;;;
+  function "suma" [natural "a"]
+  (
+   code(
+    For("i":n=0 ; "i"<'"a" ; "i" :n= "i" +' 1)
+    {
+     "s" :n= "s" +' "a"
+    }
+  )
+  ) ;;;
+  (struct "pereche"
+  [
+    member "stanga" default_nat;
+    member "dreapta" default_nat
+  ]);;;
+
+  main 
+      ("a" :n= 10 ;;
+       "n" :n= 10 ;;
+      "ok" :b= btrue ;;
+      "i" :n= 0 ;;
+      "msg" :s= "Hello" ;;
+      "nume" :s= "Ana" += "Maria" ;;
+      "suma" {{[variable "a"]}};;
+      switch (avar "a")
+     [case (5) ("a" :n= 4);
+     defaultcase ("a" :n= 0)];;
+      while ("i" <' "n" +' 1) (
+            "s" :n= "s" +' 1 ;;
+            "i" :n= "i" +' 1
+      )
+).
+Compute prg.
 
-(*SEMANTICS*)
-
-Definition check_eq_over_types (t1 : Value) (t2 : Value) : bool :=
-  match t1 with
-    | undeclared => match t2 with 
-                     | undeclared => true
-                     | _ => false
-                     end
-    | default => match t2 with 
-                  | default => true
-                  | _ => false
-                  end
-    | err_assign => match t2 with 
-                  | err_assign => true
-                  | _ => false
-                  end
-    | nat_value _x => match t2 with
-                  | nat_value _x => true
-                  | _ => false
-                  end
-    | bool_value _x => match t2 with 
-                  | bool_value _x => true
-                  | _ => false
-                  end
-    | string_value  _x => match t2 with
-                  | string_value _x => true
-                  | _ => false
-                  end
-    | code _x => match t2 with
-                  | code _x => true
-                  | _ => false
-                 end
-  end. 
-
-Inductive Mem :=
-  | mem_default : Mem
-  | offset : nat -> Mem. (* offset which indicates the current number of memory zones *)
-
-Scheme Equality for Mem.
-
-(* Environment *)
-Definition Env := string -> Mem.
-
-(* Memory Layer *)
-Definition MemLayer := Mem -> Value.
-
-(*  Notation "S [ V /' X ]" := (update S X V) (at level 20). *)
-
-(* Definition Memory := nat -> Value. *)
-
-(* Stack *)
-Definition Stack := list Env.
-
-(* Configuration *)
-Inductive Config :=
-  | config : nat -> Env -> MemLayer -> Stack -> Config.
-
-
-Definition env : Env := fun x => mem_default.
-Definition mem : MemLayer := fun x => undeclared.
-Definition stack : Stack := [env].
-
-(* Pay attention!!! In order to be able to monitor the state of the entire program, you need to
-   implement a function "update_conf", which updates the 
-   entire configuration (environment, memory layout and stack).  
-   config : nat -> Env -> MemLayer -> Stack -> Config (the first value represents the last memory zone, 
-   and you will need to find a way to increment it each time a new variable/function is declared)
-*)
-
-(* Definition update_conf_nat (n:nat) (c:Config) : Config :=
-  match c with
-  | config n' e m s => config (n+n') e m s
-  end.  *)
-
-Definition update_conf (n:nat) (env : Env) (mem:MemLayer) (s:Stack) (c:Config) : Config :=
-  match c with
-  | config a b c d => config (n+a) env mem (env :: d)
-  end.
-
-Compute update_conf 1 env mem stack.
-
-
-(* Function for updating the environment *)
-Definition update_env (env: Env) (x: string) (n: Mem) : Env :=
-  fun y =>
-      (* If the variable has assigned a default memory zone, 
-         then it will be updated with the current memory offset *)
-      if (andb (string_beq x y ) (Mem_beq (env y) mem_default))
-      then
-        n
-      else
-        (env y).
-
-Notation "S [ V /e X ]" := (update_env S X V) (at level 10). 
-
-(* Initially each variable is assigned to a default memory zone *)
-Compute (env "z"). (* The variable is not yet declared *)
-Compute mem (env "z").
-Compute mem (offset 0).
-
-(* Example of updating the environment, based on a specific memory offset *)
-Compute (update_env env "x" (offset 9)) "x".
-
-(* Function for updating the memory layer *)
-Definition update_mem (mem : MemLayer) (env : Env) (x : string) (type : Mem) (v : Value) : MemLayer :=
-  fun y => 
-      if(andb (Mem_beq (env x) type) (Mem_beq y type))
-      then
-        if(andb(check_eq_over_types undeclared (mem y)) (negb(check_eq_over_types default v)))
-        then undeclared
-        else if (andb (check_eq_over_types undeclared (mem y)) (check_eq_over_types default v))
-            then default
-            else if(orb(check_eq_over_types default (mem y)) (check_eq_over_types v (mem y)))
-                 then v
-                 else err_assign
-      else (mem y).
-Notation "S { V /m X } \ M \ T" := (update_mem M S V T X)(at level 10).
-Check env [ (offset 4) /e "a" ].
-Check env {"a" /m (nat_value 10)}\mem\(mem_default).
-
-(*AEXP SEMANTICS*)
-
-
-Definition plus_ErrorNat (n1 n2 : ErrorNat) : ErrorNat :=
-  match n1, n2 with
-    | error_nat, _ => error_nat
-    | _, error_nat => error_nat
-    | num v1, num v2 => num (v1 + v2)
-    end.
-
-Definition min_ErrorNat (n1 n2 : ErrorNat) : ErrorNat :=
-  match n1, n2 with
-    | error_nat, _ => error_nat
-    | _, error_nat => error_nat
-    | num n1, num n2 => if Nat.ltb n1 n2
-                        then error_nat
-                        else num (n1 - n2)
-    end.
-
-Definition mul_ErrorNat (n1 n2 : ErrorNat) : ErrorNat :=
-  match n1, n2 with
-    | error_nat, _ => error_nat
-    | _, error_nat => error_nat
-    | num v1, num v2 => num (v1 * v2)
-    end.
-
-Definition div_ErrorNat (n1 n2 : ErrorNat) : ErrorNat :=
-  match n1, n2 with
-    | error_nat, _ => error_nat
-    | _, error_nat => error_nat
-    | _, num 0 => error_nat
-    | num v1, num v2 => num (Nat.div v1 v2)
-    end.
-
-Definition mod_ErrorNat (n1 n2 : ErrorNat) : ErrorNat :=
-  match n1, n2 with
-    | error_nat, _ => error_nat
-    | _, error_nat => error_nat
-    | _, num 0 => error_nat
-    | num v1, num v2 => num (v1 - v2 * (Nat.div v1 v2))
-    end.
-
-(* Fixpoint aeval_fun (a : AExp) (env : Env) (mem:MemLayer) : ErrorNat :=
-  match a with
-  | avar v => match (mem (env v)) with
-                | nat_value n => n
-                | _ => error_nat
-                end
-  | anum v => v
-  | aplus a1 a2 => (plus_ErrorNat (aeval_fun a1 env mem) (aeval_fun a2 env mem))
-  | amul a1 a2 => (mul_ErrorNat (aeval_fun a1 env mem) (aeval_fun a2 env mem))
-  | amin a1 a2 => (min_ErrorNat (aeval_fun a1 env mem) (aeval_fun a2 env mem))
-  | adiv a1 a2 => (div_ErrorNat  (aeval_fun a1 env mem) (aeval_fun a2 env mem))
-  | amod a1 a2 => (mod_ErrorNat (aeval_fun a1 env mem) (aeval_fun a2 env mem))
-  end.
- *)
-
-Reserved Notation "A ` M =[ S ]=> N" (at level 30).
-
-Inductive aeval : AExp -> Env -> MemLayer -> ErrorNat -> Prop :=
-| const : forall n sigma mem , anum n ` mem =[ sigma ]=> n (* <n,sigma> => <n> *) 
-| var : forall v sigma mem ,avar v ` mem =[ sigma ]=>  match (mem (sigma v)) with
-                                                     | nat_value x => x
-                                                     | _ => error_nat
-                                                      end
-| add : forall a1 a2 i1 i2 sigma n,
-    a1 ` mem=[ sigma ]=> i1 ->
-    a2 ` mem =[ sigma ]=> i2 ->
-    n = (plus_ErrorNat i1 i2) ->
-    (a1 +' a2) ` mem =[sigma]=> n
-| diff: forall a1 a2 i1 i2 sigma n,
-    a1 ` mem =[ sigma ]=> i1 ->
-    a2 ` mem =[ sigma ]=> i2 ->
-    n = (min_ErrorNat i1 i2) ->
-    (a1 -' a2) ` mem=[sigma]=> n
-| times : forall a1 a2 i1 i2 sigma n,
-    a1 ` mem =[ sigma ]=> i1 ->
-    a2 ` mem =[ sigma ]=> i2 ->
-    n = (mul_ErrorNat i1 i2) ->
-    (a1 *' a2) ` mem =[sigma]=> n
-| div : forall a1 a2 i1 i2 sigma n,
-    a1 ` mem=[ sigma ]=> i1 ->
-    a2 ` mem=[ sigma ]=> i2 ->
-    n = (div_ErrorNat i1 i2) ->
-    (a1 /' a2) ` mem =[sigma]=> n
-| modulo : forall a1 a2 i1 i2 sigma n,
-    a1 ` mem=[ sigma ]=> i1 ->
-    a2 ` mem=[ sigma ]=> i2 ->
-    n = (mod_ErrorNat i1 i2) ->
-    (a1 %' a2) ` mem=[sigma]=> n
-where "a ` mem =[ sigma ]=> n" := (aeval a sigma mem n).
-
-
-Example division_error : (12 /' 0) ` mem =[ env ]=> error_nat.
-Proof.
-  eapply div.
-  - apply const.
-  - apply const.
-  - simpl. reflexivity.
-Qed.
-
-Example diff1 : (13 -' 5) ` mem =[ env ]=> 8.
-Proof.
-  eapply diff.
-  -apply const.
-  -apply const.
-  -simpl. reflexivity.
-Qed.
-
-(* BEXP SEMANTICS *)
-
-
-Definition lt_ErrorBool (n1 n2 : ErrorNat) : ErrorBool :=
-  match n1, n2 with
-    | error_nat, _ => error_bool
-    | _, error_nat => error_bool
-    | num v1, num v2 => boolean (Nat.ltb v1 v2)
-    end.
-
-Definition gt_ErrorBool (n1 n2 : ErrorNat) : ErrorBool :=
-  match n1, n2 with
-    | error_nat, _ => error_bool
-    | _, error_nat => error_bool
-    | num v1, num v2 => boolean (negb (Nat.ltb v1 v2))
-    end.
-
-Definition not_ErrorBool (n :ErrorBool) : ErrorBool :=
-  match n with
-    | error_bool => error_bool
-    | boolean v => boolean (negb v)
-    end.
-
-Definition and_ErrorBool (n1 n2 : ErrorBool) : ErrorBool :=
-  match n1, n2 with
-    | error_bool, _ => error_bool
-    | _, error_bool => error_bool
-    | boolean v1, boolean v2 => boolean (andb v1 v2)
-    end.
-
-Definition or_ErrorBool (n1 n2 : ErrorBool) : ErrorBool :=
-  match n1, n2 with
-    | error_bool, _ => error_bool
-    | _, error_bool => error_bool
-    | boolean v1, boolean v2 => boolean (orb v1 v2)
-    end.
-
-(* Fixpoint beval_fun (a : BExp) (envnat : Env) (mem : MemLayer) : ErrorBool :=
-  match a with
-  | btrue => true
-  | bfalse => false
-  | berror => error_bool
-  | bvar v => match mem(env v) with
-                |  bool_value n => n
-                | _ => error_bool
-                end
-  | blessthan a1 a2 => (lt_ErrorBool (aeval_fun a1 envnat mem) (aeval_fun a2 envnat mem))
-  | bgreaterthan a1 a2 => (gt_ErrorBool (aeval_fun a1 envnat mem ) (aeval_fun a2 envnat mem))
-  | bnot b1 => (not_ErrorBool (beval_fun b1 envnat mem))
-  | band b1 b2 => (and_ErrorBool (beval_fun b1 envnat mem) (beval_fun b2 envnat mem))
-  | bor b1 b2 => (or_ErrorBool (beval_fun b1 envnat mem) (beval_fun b2 envnat mem))
-  end. *)
-
-Reserved Notation "B ~' M ={ S }=> B'" (at level 20).
-Inductive beval : BExp -> Env -> ErrorBool -> MemLayer -> Prop :=
-| b_error: forall sigma mem, berror ~' mem ={ sigma }=> error_bool
-| b_true : forall sigma mem, btrue ~' mem ={ sigma }=> true
-| b_false : forall sigma mem, bfalse  ~' mem ={ sigma }=>   false
-| b_var : forall v sigma mem, bvar v  ~' mem ={ sigma }=>   match mem(sigma v) with
-                                                | bool_value x => x
-                                                | _ => error_bool
-                                                end
-| b_lessthan : forall a1 a2 i1 i2 sigma b mem,
-    a1 ` mem =[ sigma ]=> i1 ->
-    a2 ` mem =[ sigma ]=> i2 ->
-    b = (lt_ErrorBool i1 i2) ->
-    (a1 <' a2)  ~' mem ={ sigma }=>   b
-| b_not : forall a1 i1 sigma b mem,
-    a1 ~' mem ={ sigma }=> i1 ->
-    b = (not_ErrorBool i1) ->
-    (!'a1)  ~' mem ={ sigma }=>   b 
-| b_and : forall a1 a2 i1 i2 sigma b,
-    a1  ~' mem ={ sigma }=> i1 ->
-    a2  ~' mem ={ sigma }=> i2 ->
-    b = (and_ErrorBool i1 i2) ->
-    (a1 and' a2)  ~' mem ={ sigma }=>  b
-| b_or : forall a1 a2 i1 i2 sigma b,
-    a1 ~' mem ={ sigma }=> i1 ->
-    a2 ~' mem ={ sigma }=> i2 ->
-    b = (or_ErrorBool i1 i2) ->
-    (a1 or' a2)  ~' mem ={ sigma }=>  b 
-where "B ~' M ={ S }=> B'" := (beval B S B' M).
-
-(* add examples *)
-
-
-(* STRING OPERATIONS SEMANTICS *)
-
-Definition concat_ErrorString (s1 s2 : ErrorString ) : ErrorString :=
-  match s1, s2 with 
-  | error_string,_ => error_string
-  | _,error_string => error_string
-  | String s1, String s2 => String (append s1 s2)
-  end.
-
-Definition areEqual_ErrorString (s1 s2 : ErrorString) : ErrorString :=
-  match s1, s2 with
-  | error_string,_ => error_string
-  | _,error_string => error_string
-  | String s1, String s2 => if (eqb s1 s2 )
-                            then s1
-                            else String (EmptyString)
-  end.
-
-(* Definition substring_ErrorString (s1 : ErrorString) (n m:AExp) : StringExp :=
-  match s1 with
-  | error_string =>sstring error_string  
-  | String s1 =>  (substring s1 n m)
-  end. *)
-
-(* Fixpoint seval_fun (s:StringExp)(env:Env)(mem:MemLayer) : ErrorString :=
-  match s with
-  | svar s1 => match (mem(env s1)) with
-              | string_value a => a
-              | _ => error_string
-               end
-  | sstring s1 => s1
-  | strcat s1 s2 => (concat_ErrorString (seval_fun s1 env mem) (seval_fun s2 env mem)) 
-  | areEqual s1 s2 => (areEqual_ErrorString (seval_fun s1 env mem) (seval_fun s2 env mem))
-  end.
- *)
-(* 
-Inductive seval: StringExp -> Env -> MemLayer -> ErrorString -> Prop :=
-| Svar: forall s sigma mem, seval (svar s) sigma mem s
-| Sstring: forall s sigma mem, seval (sstring s) sigma mem match(mem(sigma s)) with
-                                                          | string_value s => s
-                                                          | _ => error_string
-                                                          end.
-
- *)
-
-(*STATEMENTS SEMANTICS*)
-
-
-Definition getFromConfigEnv (c:Config) : Env :=
-match c with
-| config a b c d => b
-end.
-
-Definition getFromConfigMemZone (c:Config) : nat :=
-match c with
-| config a b c d => a
-end.
-
-Definition getFromConfigMem (c:Config) : MemLayer :=
-match c with 
-| config a b c d => c
-end.
-
-Definition getFromConfigStack (c:Config) : Stack :=
-match c with 
-| config a b c d => d
-end. 
-
-
-(* Fixpoint eval_fun (s : Stmt) (gas: nat) (config' :Config) : Config :=
-    match gas with
-    | 0 => config'
-    | S gas' => match s with
-                | sequence S1 S2 => eval_fun S2 gas' (eval_fun S1 gas' config') 
-                | nat_decl a aexp => update_conf 1 (update_env (getFromConfigEnv config') a (offset (getFromConfigMemZone config'))) (update_mem (getFromConfigMem config') (getFromConfigEnv config') a (offset(getFromConfigMemZone config')) ((nat_value (aeval_fun aexp env (getFromConfigMem config')))))(getFromConfigStack config') config'
-                | bool_decl b bexp => config'
-                | string_decl s StringExp => config'
-                | array_decl s n => config'
-                | array_decl_list_nat s n l => config'
-                | array_decl_list_bool s n l => config'
-| array_decl_list_string s n l => config'
-| pointer_decl_nat s p => config'
-| pointer_decl_bool s p => config'
-| reference_decl s s' => config'
-| nat_assign s a => config'
-| bool_assign s b => config'
-| string_assign s a => config'
-| pointer_assign s p => config'
-| reference_assign s a => config'
-| array_elm_assign_nat a n => config'
-| array_elm_assign_bool a b => config'
-| array_elm_assign_string a s => config'
-| ifthen b s => config'
-| ifthenelse b s1 s2 => config'
-| while b s => config'
-| For s1 b s2 s3 => config'
-| switch a l => config'
-| functionCall s l => config'
-
-              end    
-end.
-
-
-Compute (eval_fun ("a" :n= 5) 10 (config 1 env mem stack)(getFromConfigEnv (eval_fun ("a" :n= 5) 10 (config 1 env mem stack)) "a")).
- 
-
-Reserved Notation "S \ C -{ Sigma }-> Sigma'" (at level 60).
-
-Inductive eval : Stmt -> Env -> Config -> Env -> Prop :=
-| e_nat_decl: forall a i x c sigma sigma',
-   a =[ sigma ]=> i ->
-   sigma' = (update sigma x (res_nat i)) ->
-   (x :n= a) -{ sigma }-> sigma' *)
-(* 
-| e_nat_assign: forall a i x sigma sigma',
-    a =[ sigma ]=> i ->
-    sigma' = (update sigma x (res_nat i)) ->
-    (x :n= a) -{ sigma }-> sigma'
-| e_bool_decl: forall a i x sigma sigma',
-   a ={ sigma }=> i ->
-   sigma' = (update sigma x (res_bool i)) ->
-   (x :b= a) -{ sigma }-> sigma'
-| e_bool_assign: forall a i x sigma sigma',
-    a ={ sigma }=> i ->
-    sigma' = (update sigma x (res_bool i)) ->
-    (x :b= a) -{ sigma }-> sigma'
-| e_seq : forall s1 s2 sigma sigma1 sigma2,
-    s1 -{ sigma }-> sigma1 ->
-    s2 -{ sigma1 }-> sigma2 ->
-    (s1 ;; s2) -{ sigma }-> sigma2
-| e_if_then : forall b s sigma,
-    ifthen b s -{ sigma }-> sigma
-| e_if_then_elsetrue : forall b s1 s2 sigma sigma',
-    b ={ sigma }=> true ->
-    s1 -{ sigma }-> sigma' ->
-    ifthenelse b s1 s2 -{ sigma }-> sigma' 
-| e_if_then_elsefalse : forall b s1 s2 sigma sigma',
-    b ={ sigma }=> false ->
-    s2 -{ sigma }-> sigma' ->
-    ifthenelse b s1 s2 -{ sigma }-> sigma' 
-| e_whilefalse : forall b s sigma,
-    b ={ sigma }=> false ->
-    while b s -{ sigma }-> sigma
-| e_whiletrue : forall b s sigma sigma',
-    b ={ sigma }=> true ->
-    (s ;; while b s) -{ sigma }-> sigma' ->
-    while b s -{ sigma }-> sigma' 
-where "s \ config -{ sigma }-> sigma'" := (eval s sigma config sigma').*)
 
