semantica.v
@@ -1,0 +1,467 @@
+Load proiect.
+
+
+(*SEMANTICS*)
+
+Definition check_eq_over_types (t1 : Value) (t2 : Value) : bool :=
+  match t1 with
+    | undeclared => match t2 with 
+                     | undeclared => true
+                     | _ => false
+                     end
+    | default => match t2 with 
+                  | default => true
+                  | _ => false
+                  end
+    | err_assign => match t2 with 
+                  | err_assign => true
+                  | _ => false
+                  end
+    | nat_value _x => match t2 with
+                  | nat_value _x => true
+                  | _ => false
+                  end
+    | bool_value _x => match t2 with 
+                  | bool_value _x => true
+                  | _ => false
+                  end
+    | string_value  _x => match t2 with
+                  | string_value _x => true
+                  | _ => false
+                  end
+    | code _x => match t2 with
+                  | code _x => true
+                  | _ => false
+                 end
+  end. 
+
+Inductive Mem :=
+  | mem_default : Mem
+  | offset : nat -> Mem. (* offset which indicates the current number of memory zones *)
+
+Scheme Equality for Mem.
+
+(* Environment *)
+Definition Env := string -> Mem.
+
+(* Memory Layer *)
+Definition MemLayer := Mem -> Value.
+
+(*  Notation "S [ V /' X ]" := (update S X V) (at level 20). *)
+
+(* Definition Memory := nat -> Value. *)
+
+(* Stack *)
+Definition Stack := list Env.
+
+(* Configuration *)
+Inductive Config :=
+  | config : nat -> Env -> MemLayer -> Stack -> Config.
+
+
+Definition env : Env := fun x => mem_default.
+Definition mem : MemLayer := fun x => undeclared.
+Definition stack : Stack := [env].
+
+(* Pay attention!!! In order to be able to monitor the state of the entire program, you need to
+   implement a function "update_conf", which updates the 
+   entire configuration (environment, memory layout and stack).  
+   config : nat -> Env -> MemLayer -> Stack -> Config (the first value represents the last memory zone, 
+   and you will need to find a way to increment it each time a new variable/function is declared)
+*)
+
+(* Definition update_conf_nat (n:nat) (c:Config) : Config :=
+  match c with
+  | config n' e m s => config (n+n') e m s
+  end.  *)
+
+Definition update_conf (n:nat) (env : Env) (mem:MemLayer) (s:Stack) (c:Config) : Config :=
+  match c with
+  | config a b c d => config (n+a) env mem (env :: d)
+  end.
+
+Compute update_conf 1 env mem stack.
+
+
+(* Function for updating the environment *)
+Definition update_env (env: Env) (x: string) (n: Mem) : Env :=
+  fun y =>
+      (* If the variable has assigned a default memory zone, 
+         then it will be updated with the current memory offset *)
+      if (andb (string_beq x y ) (Mem_beq (env y) mem_default))
+      then
+        n
+      else
+        (env y).
+
+Notation "S [ V /e X ]" := (update_env S X V) (at level 10). 
+
+(* Initially each variable is assigned to a default memory zone *)
+Compute (env "z"). (* The variable is not yet declared *)
+Compute mem (env "z").
+Compute mem (offset 0).
+
+(* Example of updating the environment, based on a specific memory offset *)
+Compute (update_env env "x" (offset 9)) "x".
+
+(* Function for updating the memory layer *)
+Definition update_mem (mem : MemLayer) (env : Env) (x : string) (type : Mem) (v : Value) : MemLayer :=
+  fun y => 
+      if(andb (Mem_beq (env x) type) (Mem_beq y type))
+      then
+        if(andb(check_eq_over_types undeclared (mem y)) (negb(check_eq_over_types default v)))
+        then undeclared
+        else if (andb (check_eq_over_types undeclared (mem y)) (check_eq_over_types default v))
+            then default
+            else if(orb(check_eq_over_types default (mem y)) (check_eq_over_types v (mem y)))
+                 then v
+                 else err_assign
+      else (mem y).
+Notation "S { V /m X } \ M \ T" := (update_mem M S V T X)(at level 10).
+Check env [ (offset 4) /e "a" ].
+Check env {"a" /m (nat_value 10)}\mem\(mem_default).
+
+(*AEXP SEMANTICS*)
+
+
+Definition plus_ErrorNat (n1 n2 : ErrorNat) : ErrorNat :=
+  match n1, n2 with
+    | error_nat, _ => error_nat
+    | _, error_nat => error_nat
+    | num v1, num v2 => num (v1 + v2)
+    end.
+
+Definition min_ErrorNat (n1 n2 : ErrorNat) : ErrorNat :=
+  match n1, n2 with
+    | error_nat, _ => error_nat
+    | _, error_nat => error_nat
+    | num n1, num n2 => if Nat.ltb n1 n2
+                        then error_nat
+                        else num (n1 - n2)
+    end.
+
+Definition mul_ErrorNat (n1 n2 : ErrorNat) : ErrorNat :=
+  match n1, n2 with
+    | error_nat, _ => error_nat
+    | _, error_nat => error_nat
+    | num v1, num v2 => num (v1 * v2)
+    end.
+
+Definition div_ErrorNat (n1 n2 : ErrorNat) : ErrorNat :=
+  match n1, n2 with
+    | error_nat, _ => error_nat
+    | _, error_nat => error_nat
+    | _, num 0 => error_nat
+    | num v1, num v2 => num (Nat.div v1 v2)
+    end.
+
+Definition mod_ErrorNat (n1 n2 : ErrorNat) : ErrorNat :=
+  match n1, n2 with
+    | error_nat, _ => error_nat
+    | _, error_nat => error_nat
+    | _, num 0 => error_nat
+    | num v1, num v2 => num (v1 - v2 * (Nat.div v1 v2))
+    end.
+
+(* Fixpoint aeval_fun (a : AExp) (env : Env) (mem:MemLayer) : ErrorNat :=
+  match a with
+  | avar v => match (mem (env v)) with
+                | nat_value n => n
+                | _ => error_nat
+                end
+  | anum v => v
+  | aplus a1 a2 => (plus_ErrorNat (aeval_fun a1 env mem) (aeval_fun a2 env mem))
+  | amul a1 a2 => (mul_ErrorNat (aeval_fun a1 env mem) (aeval_fun a2 env mem))
+  | amin a1 a2 => (min_ErrorNat (aeval_fun a1 env mem) (aeval_fun a2 env mem))
+  | adiv a1 a2 => (div_ErrorNat  (aeval_fun a1 env mem) (aeval_fun a2 env mem))
+  | amod a1 a2 => (mod_ErrorNat (aeval_fun a1 env mem) (aeval_fun a2 env mem))
+  end.
+ *)
+
+Reserved Notation "A ` M =[ S ]=> N" (at level 30).
+
+Inductive aeval : AExp -> Env -> MemLayer -> ErrorNat -> Prop :=
+| const : forall n sigma mem , anum n ` mem =[ sigma ]=> n (* <n,sigma> => <n> *) 
+| var : forall v sigma mem ,avar v ` mem =[ sigma ]=>  match (mem (sigma v)) with
+                                                     | nat_value x => x
+                                                     | _ => error_nat
+                                                      end
+| add : forall a1 a2 i1 i2 sigma n,
+    a1 ` mem=[ sigma ]=> i1 ->
+    a2 ` mem =[ sigma ]=> i2 ->
+    n = (plus_ErrorNat i1 i2) ->
+    (a1 +' a2) ` mem =[sigma]=> n
+| diff: forall a1 a2 i1 i2 sigma n,
+    a1 ` mem =[ sigma ]=> i1 ->
+    a2 ` mem =[ sigma ]=> i2 ->
+    n = (min_ErrorNat i1 i2) ->
+    (a1 -' a2) ` mem=[sigma]=> n
+| times : forall a1 a2 i1 i2 sigma n,
+    a1 ` mem =[ sigma ]=> i1 ->
+    a2 ` mem =[ sigma ]=> i2 ->
+    n = (mul_ErrorNat i1 i2) ->
+    (a1 *' a2) ` mem =[sigma]=> n
+| div : forall a1 a2 i1 i2 sigma n,
+    a1 ` mem=[ sigma ]=> i1 ->
+    a2 ` mem=[ sigma ]=> i2 ->
+    n = (div_ErrorNat i1 i2) ->
+    (a1 /' a2) ` mem =[sigma]=> n
+| modulo : forall a1 a2 i1 i2 sigma n,
+    a1 ` mem=[ sigma ]=> i1 ->
+    a2 ` mem=[ sigma ]=> i2 ->
+    n = (mod_ErrorNat i1 i2) ->
+    (a1 %' a2) ` mem=[sigma]=> n
+where "a ` mem =[ sigma ]=> n" := (aeval a sigma mem n).
+
+
+Example division_error : (12 /' 0) ` mem =[ env ]=> error_nat.
+Proof.
+  eapply div.
+  - apply const.
+  - apply const.
+  - simpl. reflexivity.
+Qed.
+
+Example diff1 : (13 -' 5) ` mem =[ env ]=> 8.
+Proof.
+  eapply diff.
+  -apply const.
+  -apply const.
+  -simpl. reflexivity.
+Qed.
+
+(* BEXP SEMANTICS *)
+
+
+Definition lt_ErrorBool (n1 n2 : ErrorNat) : ErrorBool :=
+  match n1, n2 with
+    | error_nat, _ => error_bool
+    | _, error_nat => error_bool
+    | num v1, num v2 => boolean (Nat.ltb v1 v2)
+    end.
+
+Definition gt_ErrorBool (n1 n2 : ErrorNat) : ErrorBool :=
+  match n1, n2 with
+    | error_nat, _ => error_bool
+    | _, error_nat => error_bool
+    | num v1, num v2 => boolean (negb (Nat.ltb v1 v2))
+    end.
+
+Definition not_ErrorBool (n :ErrorBool) : ErrorBool :=
+  match n with
+    | error_bool => error_bool
+    | boolean v => boolean (negb v)
+    end.
+
+Definition and_ErrorBool (n1 n2 : ErrorBool) : ErrorBool :=
+  match n1, n2 with
+    | error_bool, _ => error_bool
+    | _, error_bool => error_bool
+    | boolean v1, boolean v2 => boolean (andb v1 v2)
+    end.
+
+Definition or_ErrorBool (n1 n2 : ErrorBool) : ErrorBool :=
+  match n1, n2 with
+    | error_bool, _ => error_bool
+    | _, error_bool => error_bool
+    | boolean v1, boolean v2 => boolean (orb v1 v2)
+    end.
+
+(* Fixpoint beval_fun (a : BExp) (envnat : Env) (mem : MemLayer) : ErrorBool :=
+  match a with
+  | btrue => true
+  | bfalse => false
+  | berror => error_bool
+  | bvar v => match mem(env v) with
+                |  bool_value n => n
+                | _ => error_bool
+                end
+  | blessthan a1 a2 => (lt_ErrorBool (aeval_fun a1 envnat mem) (aeval_fun a2 envnat mem))
+  | bgreaterthan a1 a2 => (gt_ErrorBool (aeval_fun a1 envnat mem ) (aeval_fun a2 envnat mem))
+  | bnot b1 => (not_ErrorBool (beval_fun b1 envnat mem))
+  | band b1 b2 => (and_ErrorBool (beval_fun b1 envnat mem) (beval_fun b2 envnat mem))
+  | bor b1 b2 => (or_ErrorBool (beval_fun b1 envnat mem) (beval_fun b2 envnat mem))
+  end. *)
+
+Reserved Notation "B ~' M ={ S }=> B'" (at level 20).
+Inductive beval : BExp -> Env -> ErrorBool -> MemLayer -> Prop :=
+| b_error: forall sigma mem, berror ~' mem ={ sigma }=> error_bool
+| b_true : forall sigma mem, btrue ~' mem ={ sigma }=> true
+| b_false : forall sigma mem, bfalse  ~' mem ={ sigma }=>   false
+| b_var : forall v sigma mem, bvar v  ~' mem ={ sigma }=>   match mem(sigma v) with
+                                                | bool_value x => x
+                                                | _ => error_bool
+                                                end
+| b_lessthan : forall a1 a2 i1 i2 sigma b mem,
+    a1 ` mem =[ sigma ]=> i1 ->
+    a2 ` mem =[ sigma ]=> i2 ->
+    b = (lt_ErrorBool i1 i2) ->
+    (a1 <' a2)  ~' mem ={ sigma }=>   b
+| b_not : forall a1 i1 sigma b mem,
+    a1 ~' mem ={ sigma }=> i1 ->
+    b = (not_ErrorBool i1) ->
+    (!'a1)  ~' mem ={ sigma }=>   b 
+| b_and : forall a1 a2 i1 i2 sigma b,
+    a1  ~' mem ={ sigma }=> i1 ->
+    a2  ~' mem ={ sigma }=> i2 ->
+    b = (and_ErrorBool i1 i2) ->
+    (a1 and' a2)  ~' mem ={ sigma }=>  b
+| b_or : forall a1 a2 i1 i2 sigma b,
+    a1 ~' mem ={ sigma }=> i1 ->
+    a2 ~' mem ={ sigma }=> i2 ->
+    b = (or_ErrorBool i1 i2) ->
+    (a1 or' a2)  ~' mem ={ sigma }=>  b 
+where "B ~' M ={ S }=> B'" := (beval B S B' M).
+
+(* add examples *)
+
+
+(* STRING OPERATIONS SEMANTICS *)
+
+Definition concat_ErrorString (s1 s2 : ErrorString ) : ErrorString :=
+  match s1, s2 with 
+  | error_string,_ => error_string
+  | _,error_string => error_string
+  | String s1, String s2 => String (append s1 s2)
+  end.
+
+Definition areEqual_ErrorString (s1 s2 : ErrorString) : ErrorString :=
+  match s1, s2 with
+  | error_string,_ => error_string
+  | _,error_string => error_string
+  | String s1, String s2 => if (eqb s1 s2 )
+                            then s1
+                            else String (EmptyString)
+  end.
+
+(* Definition substring_ErrorString (s1 : ErrorString) (n m:AExp) : StringExp :=
+  match s1 with
+  | error_string =>sstring error_string  
+  | String s1 =>  (substring s1 n m)
+  end. *)
+
+(* Fixpoint seval_fun (s:StringExp)(env:Env)(mem:MemLayer) : ErrorString :=
+  match s with
+  | svar s1 => match (mem(env s1)) with
+              | string_value a => a
+              | _ => error_string
+               end
+  | sstring s1 => s1
+  | strcat s1 s2 => (concat_ErrorString (seval_fun s1 env mem) (seval_fun s2 env mem)) 
+  | areEqual s1 s2 => (areEqual_ErrorString (seval_fun s1 env mem) (seval_fun s2 env mem))
+  end.
+ *)
+(* 
+Inductive seval: StringExp -> Env -> MemLayer -> ErrorString -> Prop :=
+| Svar: forall s sigma mem, seval (svar s) sigma mem s
+| Sstring: forall s sigma mem, seval (sstring s) sigma mem match(mem(sigma s)) with
+                                                          | string_value s => s
+                                                          | _ => error_string
+                                                          end.
+
+ *)
+
+(*STATEMENTS SEMANTICS*)
+
+
+Definition getFromConfigEnv (c:Config) : Env :=
+match c with
+| config a b c d => b
+end.
+
+Definition getFromConfigMemZone (c:Config) : nat :=
+match c with
+| config a b c d => a
+end.
+
+Definition getFromConfigMem (c:Config) : MemLayer :=
+match c with 
+| config a b c d => c
+end.
+
+Definition getFromConfigStack (c:Config) : Stack :=
+match c with 
+| config a b c d => d
+end. 
+
+
+(* Fixpoint eval_fun (s : Stmt) (gas: nat) (config' :Config) : Config :=
+    match gas with
+    | 0 => config'
+    | S gas' => match s with
+                | sequence S1 S2 => eval_fun S2 gas' (eval_fun S1 gas' config') 
+                | nat_decl a aexp => update_conf 1 (update_env (getFromConfigEnv config') a (offset (getFromConfigMemZone config'))) (update_mem (getFromConfigMem config') (getFromConfigEnv config') a (offset(getFromConfigMemZone config')) ((nat_value (aeval_fun aexp env (getFromConfigMem config')))))(getFromConfigStack config') config'
+                | bool_decl b bexp => config'
+                | string_decl s StringExp => config'
+                | array_decl s n => config'
+                | array_decl_list_nat s n l => config'
+                | array_decl_list_bool s n l => config'
+| array_decl_list_string s n l => config'
+| pointer_decl_nat s p => config'
+| pointer_decl_bool s p => config'
+| reference_decl s s' => config'
+| nat_assign s a => config'
+| bool_assign s b => config'
+| string_assign s a => config'
+| pointer_assign s p => config'
+| reference_assign s a => config'
+| array_elm_assign_nat a n => config'
+| array_elm_assign_bool a b => config'
+| array_elm_assign_string a s => config'
+| ifthen b s => config'
+| ifthenelse b s1 s2 => config'
+| while b s => config'
+| For s1 b s2 s3 => config'
+| switch a l => config'
+| functionCall s l => config'
+
+              end    
+end.
+
+
+Compute (eval_fun ("a" :n= 5) 10 (config 1 env mem stack)(getFromConfigEnv (eval_fun ("a" :n= 5) 10 (config 1 env mem stack)) "a")).
+ 
+
+Reserved Notation "S \ C -{ Sigma }-> Sigma'" (at level 60).
+
+Inductive eval : Stmt -> Env -> Config -> Env -> Prop :=
+| e_nat_decl: forall a i x c sigma sigma',
+   a =[ sigma ]=> i ->
+   sigma' = (update sigma x (res_nat i)) ->
+   (x :n= a) -{ sigma }-> sigma' *)
+(* 
+| e_nat_assign: forall a i x sigma sigma',
+    a =[ sigma ]=> i ->
+    sigma' = (update sigma x (res_nat i)) ->
+    (x :n= a) -{ sigma }-> sigma'
+| e_bool_decl: forall a i x sigma sigma',
+   a ={ sigma }=> i ->
+   sigma' = (update sigma x (res_bool i)) ->
+   (x :b= a) -{ sigma }-> sigma'
+| e_bool_assign: forall a i x sigma sigma',
+    a ={ sigma }=> i ->
+    sigma' = (update sigma x (res_bool i)) ->
+    (x :b= a) -{ sigma }-> sigma'
+| e_seq : forall s1 s2 sigma sigma1 sigma2,
+    s1 -{ sigma }-> sigma1 ->
+    s2 -{ sigma1 }-> sigma2 ->
+    (s1 ;; s2) -{ sigma }-> sigma2
+| e_if_then : forall b s sigma,
+    ifthen b s -{ sigma }-> sigma
+| e_if_then_elsetrue : forall b s1 s2 sigma sigma',
+    b ={ sigma }=> true ->
+    s1 -{ sigma }-> sigma' ->
+    ifthenelse b s1 s2 -{ sigma }-> sigma' 
+| e_if_then_elsefalse : forall b s1 s2 sigma sigma',
+    b ={ sigma }=> false ->
+    s2 -{ sigma }-> sigma' ->
+    ifthenelse b s1 s2 -{ sigma }-> sigma' 
+| e_whilefalse : forall b s sigma,
+    b ={ sigma }=> false ->
+    while b s -{ sigma }-> sigma
+| e_whiletrue : forall b s sigma sigma',
+    b ={ sigma }=> true ->
+    (s ;; while b s) -{ sigma }-> sigma' ->
+    while b s -{ sigma }-> sigma' 
+where "s \ config -{ sigma }-> sigma'" := (eval s sigma config sigma').*)
+
